Core/Infer/Global.lean
@@ -1,0 +1,28 @@
+import Core.Infer.Kind
+import Core.Infer.Type
+
+
+def Globals.wf_globals : (G : Globals) -> Option Unit
+| .nil => return ()
+| .cons (.data (n := n) x k ctors) tl => do
+  wf_globals tl
+  let ctors' : Vec (Option Kind) n := λ i => (ctors i).snd.infer_kind ((.data x k v[]) :: tl) []
+  let _ <- ctors'.seq
+| .cons (.opent _ _) tl => do
+  wf_globals tl
+| .cons (.openm _ T) tl => do
+  wf_globals tl
+  let _ <- T.infer_kind tl []
+| .cons (.defn _ T t) tl => do
+  wf_globals tl
+  let T' <- t.infer_type tl [] []
+  let _ <- T.infer_kind tl []
+  if T == T' then return () else none
+| .cons (.inst x t) tl => do
+  wf_globals tl
+  let T <- t.infer_type tl [] []
+  let T' <- lookup_type tl x
+  if T == T' then return () else none
+| .cons (.instty _ T) tl => do
+  wf_globals tl
+  let _ <- T.infer_kind tl []
